ver2/flat_symbolic_state_eval_soundness.v
@@ -35,14 +35,14 @@ Import FlatSymbolicStateEval.
 
 
 Lemma eval_sexpr_snd:
-  forall sb sv stk mem strg ctx ops flat_sb fsv,
+  forall sb maxidx sv stk mem strg ctx ops flat_sb fsv,
     bindings_to_flat_bindings sb = Some flat_sb ->
     sstack_val_to_sexpr sv flat_sb = Some fsv ->
-    eval_sstack_val sv stk mem strg ctx sb ops = eval_sexpr fsv stk mem strg ctx ops.
+    eval_sstack_val sv stk mem strg ctx maxidx sb ops = eval_sexpr fsv stk mem strg ctx ops.
 Proof.
   induction sb as [|p sb' IHsb'].
   - simpl.
-    intros sv stk mem strg ctx ops flat_sb fsv H_bs_to_flat_bs H_sstack_val_to_sexpr.
+    intros maxidx sv stk mem strg ctx ops flat_sb fsv H_bs_to_flat_bs H_sstack_val_to_sexpr.
     injection H_bs_to_flat_bs as H_bs_to_flat_bs.
     rewrite <- H_bs_to_flat_bs in H_sstack_val_to_sexpr.
     simpl in H_sstack_val_to_sexpr.
@@ -51,7 +51,7 @@ Proof.
       rewrite <- H_sstack_val_to_sexpr;
       simpl;
       reflexivity) || discriminate.
-  - intros sv stk mem strg ctx ops flat_sb fsv H_bs_to_flat_bs H_sstack_val_to_sexpr.
+  - intros maxidx sv stk mem strg ctx ops flat_sb fsv H_bs_to_flat_bs H_sstack_val_to_sexpr.
     
     destruct sv; try (
                      simpl;
@@ -110,7 +110,7 @@ Proof.
         destruct (length args =? nrags) eqn:E_len_args_nargs.
         ++ destruct (length sexpr_args =? nrags) eqn:E_len_sexpr_nargs.
            +++ fold eval_sexpr.
-               assert (H_maps_option_aux: forall args sexpr_args, map_option (fun sv' : sstack_val => sstack_val_to_sexpr sv' flat_sb') args = Some sexpr_args -> map_option (fun sv' : sstack_val => eval_sstack_val sv' stk mem strg ctx sb' ops) args = map_option (fun fsv' : sexpr => eval_sexpr fsv' stk mem strg ctx ops) sexpr_args).
+               assert (H_maps_option_aux: forall args sexpr_args, map_option (fun sv' : sstack_val => sstack_val_to_sexpr sv' flat_sb') args = Some sexpr_args -> map_option (fun sv' : sstack_val => eval_sstack_val sv' stk mem strg ctx key sb' ops) args = map_option (fun fsv' : sexpr => eval_sexpr fsv' stk mem strg ctx ops) sexpr_args).
                (* proof of assert start *)
                ++++ intro args0. induction args0 as [| a0 args0' IHargs0'].
                     +++++ intros sexpr_args0 H_map_option_sexpr_args. simpl in H_map_option_sexpr_args. injection H_map_option_sexpr_args as H_map_option_sexpr_args. rewrite <- H_map_option_sexpr_args. simpl.  reflexivity.
@@ -122,9 +122,9 @@ Proof.
                           repeat rewrite <- map_option_ho.
 
                           assert (H_flat_sb'_refl: Some flat_sb' = Some flat_sb'). reflexivity.
-                          pose proof (IHsb' a0 stk mem strg ctx ops flat_sb' asexpr0 H_flat_sb'_refl  H_map_option_sexpr_args_1 ) as H_map_option_aux_3.
+                          pose proof (IHsb' key a0 stk mem strg ctx ops flat_sb' asexpr0 H_flat_sb'_refl  H_map_option_sexpr_args_1 ) as H_map_option_aux_3.
                           rewrite <- H_map_option_aux_3. 
-                          destruct (eval_sstack_val a0 stk mem strg ctx sb' ops); try reflexivity.
+                          destruct (eval_sstack_val a0 stk mem strg ctx key sb' ops); try reflexivity.
 
                           pose proof (IHargs0' sexpr_args0'  H_map_option_sexpr_args_2) as IHargs0'_1.
                           rewrite IHargs0'_1.
@@ -158,7 +158,7 @@ Proof.
         assert(H_map_option_0: forall smem sexpr_mem_updates,
                   map_option (eval_common.EvalCommon.instantiate_memory_update (fun sv : sstack_val => sstack_val_to_sexpr sv flat_sb')) smem = Some sexpr_mem_updates ->
                   map_option
-                    (eval_common.EvalCommon.instantiate_memory_update (fun sv : sstack_val => eval_sstack_val sv stk mem strg ctx sb' ops)) smem = map_option (eval_common.EvalCommon.instantiate_memory_update (fun sv : sexpr => eval_sexpr sv stk mem strg ctx ops)) sexpr_mem_updates). 
+                    (eval_common.EvalCommon.instantiate_memory_update (fun sv : sstack_val => eval_sstack_val sv stk mem strg ctx key sb' ops)) smem = map_option (eval_common.EvalCommon.instantiate_memory_update (fun sv : sexpr => eval_sexpr sv stk mem strg ctx ops)) sexpr_mem_updates). 
 
         (* proof of assert starts here *)
         ++ intros smem0. induction smem0 as [|supdate0 smem0' IHsmem0'].
@@ -180,9 +180,9 @@ Proof.
                                                      rewrite <- H_map_option_0_1_1;
                                                      simpl;
                
-                                                     pose proof (IHsb' offset0 stk mem strg ctx ops flat_sb' s H_flat_sb'_refl E_sstack_val_to_sexpr_offset0) as H_map_option_aux_3;
+                                                     pose proof (IHsb' key offset0 stk mem strg ctx ops flat_sb' s H_flat_sb'_refl E_sstack_val_to_sexpr_offset0) as H_map_option_aux_3;
                                                      rewrite H_map_option_aux_3;
-                                                     pose proof (IHsb' value stk mem strg ctx ops flat_sb' s0 H_flat_sb'_refl E_sstack_val_to_sexpr_value) as H_map_option_aux_4;
+                                                     pose proof (IHsb' key value stk mem strg ctx ops flat_sb' s0 H_flat_sb'_refl E_sstack_val_to_sexpr_value) as H_map_option_aux_4;
                                                      rewrite H_map_option_aux_4;
 
                                                      pose proof (IHsmem0' sexpr_mem_updates0'  H_map_option_0_1_2) as H_map_option_aux_5;
@@ -194,7 +194,7 @@ Proof.
            rewrite H_map_option_1.
 
            assert (H_flat_sb'_refl: Some flat_sb' = Some flat_sb'). reflexivity.
-           pose proof (IHsb' offset stk mem strg ctx ops flat_sb' sexpr_offset H_flat_sb'_refl E_sstack_val_to_sexpr_offset) as IHsb'_0.
+           pose proof (IHsb' key offset stk mem strg ctx ops flat_sb' sexpr_offset H_flat_sb'_refl E_sstack_val_to_sexpr_offset) as IHsb'_0.
            rewrite IHsb'_0.
            reflexivity.
       * simpl in E_smap_value_to_sexpr.
@@ -208,7 +208,7 @@ Proof.
         assert(H_map_option_0: forall sstrg sexpr_strg_updates,
                   map_option (eval_common.EvalCommon.instantiate_storage_update (fun sv : sstack_val => sstack_val_to_sexpr sv flat_sb')) sstrg = Some sexpr_strg_updates ->
                   map_option
-                    (eval_common.EvalCommon.instantiate_storage_update (fun sv : sstack_val => eval_sstack_val sv stk mem strg ctx sb' ops)) sstrg = map_option (eval_common.EvalCommon.instantiate_storage_update (fun sv : sexpr => eval_sexpr sv stk mem strg ctx ops)) sexpr_strg_updates).
+                    (eval_common.EvalCommon.instantiate_storage_update (fun sv : sstack_val => eval_sstack_val sv stk mem strg ctx key sb' ops)) sstrg = map_option (eval_common.EvalCommon.instantiate_storage_update (fun sv : sexpr => eval_sexpr sv stk mem strg ctx ops)) sexpr_strg_updates).
 
         (* proof of assert stars here *)
         ++ intros sstrg0. induction sstrg0 as [|supdate0 sstrg0' IHsstrg0'].
@@ -232,9 +232,9 @@ Proof.
                simpl.
                
                assert (H_flat_sb'_refl: Some flat_sb' = Some flat_sb'). reflexivity.
-               pose proof (IHsb' key1 stk mem strg ctx ops flat_sb' s H_flat_sb'_refl E_sstack_val_to_sexpr_key1) as H_map_option_aux_3.
+               pose proof (IHsb' key key1 stk mem strg ctx ops flat_sb' s H_flat_sb'_refl E_sstack_val_to_sexpr_key1) as H_map_option_aux_3.
                rewrite H_map_option_aux_3.
-               pose proof (IHsb' value stk mem strg ctx ops flat_sb' s0 H_flat_sb'_refl E_sstack_val_to_sexpr_value) as H_map_option_aux_4.
+               pose proof (IHsb' key value stk mem strg ctx ops flat_sb' s0 H_flat_sb'_refl E_sstack_val_to_sexpr_value) as H_map_option_aux_4.
                rewrite H_map_option_aux_4.
                
                pose proof (IHsstrg0' sexpr_strg_updates0' H_map_option_0_1_2) as H_map_option_aux_5.
@@ -246,7 +246,7 @@ Proof.
         ++ pose proof (H_map_option_0 sstrg sexpr_strg_updates E_map_option_strg_updates) as H_map_option_0_1.
            rewrite H_map_option_0_1.
            assert (H_flat_sb'_refl: Some flat_sb' = Some flat_sb'). reflexivity.
-           pose proof (IHsb' key0 stk mem strg ctx ops flat_sb' sexpr_key0 H_flat_sb'_refl E_sstack_val_to_sexpr_key0) as IHsb'_0.
+           pose proof (IHsb' key key0 stk mem strg ctx ops flat_sb' sexpr_key0 H_flat_sb'_refl E_sstack_val_to_sexpr_key0) as IHsb'_0.
            rewrite IHsb'_0.
            reflexivity.
 
@@ -266,7 +266,7 @@ Proof.
         assert(H_map_option_0: forall smem sexpr_mem_updates,
                   map_option (eval_common.EvalCommon.instantiate_memory_update (fun sv : sstack_val => sstack_val_to_sexpr sv flat_sb')) smem = Some sexpr_mem_updates ->
                   map_option
-                    (eval_common.EvalCommon.instantiate_memory_update (fun sv : sstack_val => eval_sstack_val sv stk mem strg ctx sb' ops)) smem = map_option (eval_common.EvalCommon.instantiate_memory_update (fun sv : sexpr => eval_sexpr sv stk mem strg ctx ops)) sexpr_mem_updates). 
+                    (eval_common.EvalCommon.instantiate_memory_update (fun sv : sstack_val => eval_sstack_val sv stk mem strg ctx key sb' ops)) smem = map_option (eval_common.EvalCommon.instantiate_memory_update (fun sv : sexpr => eval_sexpr sv stk mem strg ctx ops)) sexpr_mem_updates). 
 
         ++ intros smem0. induction smem0 as [|supdate0 smem0' IHsmem0'].
            +++ intros sexpr_mem_updates0 H_map_option_0_1. simpl in H_map_option_0_1. injection H_map_option_0_1 as H_map_option_0_1. rewrite <- H_map_option_0_1. simpl. reflexivity.
@@ -287,9 +287,9 @@ Proof.
                     simpl.
                
                     assert (H_flat_sb'_refl: Some flat_sb' = Some flat_sb'). reflexivity.
-                    pose proof (IHsb' offset0 stk mem strg ctx ops flat_sb' s H_flat_sb'_refl E_sstack_val_to_sexpr_offset0) as H_map_option_aux_3.
+                    pose proof (IHsb' key offset0 stk mem strg ctx ops flat_sb' s H_flat_sb'_refl E_sstack_val_to_sexpr_offset0) as H_map_option_aux_3.
                     rewrite H_map_option_aux_3.
-                    pose proof (IHsb' value stk mem strg ctx ops flat_sb' s0 H_flat_sb'_refl E_sstack_val_to_sexpr_value) as H_map_option_aux_4.
+                    pose proof (IHsb' key value stk mem strg ctx ops flat_sb' s0 H_flat_sb'_refl E_sstack_val_to_sexpr_value) as H_map_option_aux_4.
                     rewrite H_map_option_aux_4.
 
                     pose proof (IHsmem0' sexpr_mem_updates0'  H_map_option_0_1_2) as H_map_option_aux_5.
@@ -304,9 +304,9 @@ Proof.
                     simpl.
                
                     assert (H_flat_sb'_refl: Some flat_sb' = Some flat_sb'). reflexivity.
-                    pose proof (IHsb' offset0 stk mem strg ctx ops flat_sb' s H_flat_sb'_refl E_sstack_val_to_sexpr_offset0) as H_map_option_aux_3.
+                    pose proof (IHsb' key offset0 stk mem strg ctx ops flat_sb' s H_flat_sb'_refl E_sstack_val_to_sexpr_offset0) as H_map_option_aux_3.
                     rewrite H_map_option_aux_3.
-                    pose proof (IHsb' value stk mem strg ctx ops flat_sb' s0 H_flat_sb'_refl E_sstack_val_to_sexpr_value) as H_map_option_aux_4.
+                    pose proof (IHsb' key value stk mem strg ctx ops flat_sb' s0 H_flat_sb'_refl E_sstack_val_to_sexpr_value) as H_map_option_aux_4.
                     rewrite H_map_option_aux_4.
 
                     pose proof (IHsmem0' sexpr_mem_updates0'  H_map_option_0_1_2) as H_map_option_aux_5.
@@ -319,9 +319,9 @@ Proof.
            rewrite H_map_option_1.
 
            assert (H_flat_sb'_refl: Some flat_sb' = Some flat_sb'). reflexivity.
-           pose proof (IHsb' offset stk mem strg ctx ops flat_sb' sexpr_offset H_flat_sb'_refl E_sstack_val_to_sexpr_offset) as IHsb'_0.
+           pose proof (IHsb' key offset stk mem strg ctx ops flat_sb' sexpr_offset H_flat_sb'_refl E_sstack_val_to_sexpr_offset) as IHsb'_0.
            rewrite IHsb'_0.
-           pose proof (IHsb' size stk mem strg ctx ops flat_sb' sexpr_size H_flat_sb'_refl E_sstack_val_to_sexpr_size) as IHsb'_1.
+           pose proof (IHsb' key size stk mem strg ctx ops flat_sb' sexpr_size H_flat_sb'_refl E_sstack_val_to_sexpr_size) as IHsb'_1.
            rewrite IHsb'_1.
            reflexivity.
         
@@ -334,27 +334,27 @@ Proof.
 Qed.
 
 Lemma eval_sexp_map:
-  forall l flat_l sb flat_sb stk mem strg ctx ops,
+  forall l maxidx flat_l sb flat_sb stk mem strg ctx ops,
     bindings_to_flat_bindings sb = Some flat_sb ->
     map_option (fun sv : sstack_val => sstack_val_to_sexpr sv flat_sb) l = Some flat_l ->
     map_option (fun sv : sexpr => eval_sexpr sv stk mem strg ctx ops) flat_l =
-      map_option (fun sv : sstack_val => eval_sstack_val sv stk mem strg ctx sb ops) l.
+      map_option (fun sv : sstack_val => eval_sstack_val sv stk mem strg ctx maxidx sb ops) l.
 Proof.
   induction l as [|a l' IHl'].
-  - intros flat_l sb flat_sb stk mem strg ctx ops H_flat_sb H_map_option_0.
+  - intros maxidx flat_l sb flat_sb stk mem strg ctx ops H_flat_sb H_map_option_0.
     simpl in H_map_option_0.
     injection H_map_option_0 as H_map_option_0.
     rewrite <- H_map_option_0.
     simpl.
     reflexivity.
-  - intros flat_l sb flat_sb stk mem strg ctx ops H_flat_sb H_map_option_0.
+  - intros maxidx flat_l sb flat_sb stk mem strg ctx ops H_flat_sb H_map_option_0.
     pose proof (map_option_len sstack_val sexpr (fun sv : sstack_val => sstack_val_to_sexpr sv flat_sb) (a :: l') flat_l H_map_option_0) as H_map_option_1.
     destruct flat_l as [|flat_a flat_l']; try discriminate.
     pose proof (map_option_hd sstack_val sexpr (fun sv : sstack_val => sstack_val_to_sexpr sv flat_sb)  l' flat_l' a flat_a H_map_option_0) as [H_map_option_1_1 H_map_option_1_2].
-    pose proof (eval_sexpr_snd sb a stk mem strg ctx ops flat_sb flat_a H_flat_sb H_map_option_1_1) as H_eval_sexpr_snd.
+    pose proof (eval_sexpr_snd sb maxidx a stk mem strg ctx ops flat_sb flat_a H_flat_sb H_map_option_1_1) as H_eval_sexpr_snd.
     simpl.
     rewrite H_eval_sexpr_snd.
-    pose proof (IHl' flat_l' sb flat_sb stk mem strg ctx ops H_flat_sb H_map_option_1_2) as IHl'_0.
+    pose proof (IHl' maxidx flat_l' sb flat_sb stk mem strg ctx ops H_flat_sb H_map_option_1_2) as IHl'_0.
     rewrite IHl'_0.
     reflexivity.
 Qed.
@@ -382,18 +382,13 @@ Qed.
 Lemma eval_flat_sstack_snd:
   forall sst fsst stk mem strg ctx ops,
     sstate_to_flat_sstate sst = Some fsst ->
-    eval_flat_sstack stk mem strg ctx fsst ops = eval_sstack stk mem strg ctx sst ops.
+    eval_flat_sstack (get_stack_fsst fsst) stk mem strg ctx ops = eval_sstack (get_stack_sst sst) (get_maxidx_smap (get_smap_sst sst)) (get_bindings_smap (get_smap_sst sst)) stk mem strg ctx ops.
 Proof.
   intros sst fsst stk mem strg ctx ops H_sst_to_fsst.
   unfold eval_flat_sstack.
   unfold eval_sstack.
-  unfold eval_sstack'.
-  pose proof (sst_to_fsst_instk_height sst fsst H_sst_to_fsst) as H_sst_to_fsst_instk_height.
-  rewrite H_sst_to_fsst_instk_height.
-  destruct (length stk =? get_instk_height_fsst fsst) eqn:E_len_stk; try reflexivity.
-  destruct (get_smap_sst sst) as [maxid sb] eqn:E_get_smap.
   unfold sstate_to_flat_sstate in H_sst_to_fsst.
-  rewrite E_get_smap in H_sst_to_fsst.
+  destruct (get_smap_sst sst) as [maxidx sb] eqn:E_get_smap.
   destruct (bindings_to_flat_bindings sb) as [flat_sb|] eqn:E_bindings; try discriminate.
   destruct (sstack_to_flat_sstack sst flat_sb) as [flat_sstk|] eqn:E_flat_sstk; try discriminate.
   destruct (smemory_to_flat_smemory sst flat_sb) as [flat_smem|] eqn:E_flat_smem; try discriminate.
@@ -403,19 +398,19 @@ Proof.
   simpl in H_sst_to_fsst.
   rewrite <- H_sst_to_fsst.
   simpl.
-  pose proof (eval_sexp_map (get_stack_sst sst) flat_sstk sb flat_sb stk mem strg ctx ops E_bindings E_flat_sstk) as H_eval_sexp_map.
+  pose proof (eval_sexp_map (get_stack_sst sst) maxidx flat_sstk sb flat_sb stk mem strg ctx ops E_bindings E_flat_sstk) as H_eval_sexp_map.
   apply H_eval_sexp_map.
 Qed.
 
 Lemma eval_flat_smemory_map:
-  forall sb flat_sb stk mem strg ctx ops smem flat_smem,
+  forall sb maxidx flat_sb stk mem strg ctx ops smem flat_smem,
     bindings_to_flat_bindings sb = Some flat_sb ->
     map_option (eval_common.EvalCommon.instantiate_memory_update (fun sv : sstack_val => sstack_val_to_sexpr sv flat_sb)) smem = Some flat_smem ->
 
   map_option (eval_common.EvalCommon.instantiate_memory_update (fun sv : sexpr => eval_sexpr sv stk mem strg ctx ops)) flat_smem =
-    map_option (eval_common.EvalCommon.instantiate_memory_update (fun sv : sstack_val => eval_sstack_val sv stk mem strg ctx sb ops)) smem.
+    map_option (eval_common.EvalCommon.instantiate_memory_update (fun sv : sstack_val => eval_sstack_val sv stk mem strg ctx maxidx sb ops)) smem.
 Proof.
-  intros sb flat_sb stk mem strg ctx ops.
+  intros sb maxidx flat_sb stk mem strg ctx ops.
   induction smem as [|u smem' IHsmem'].
   - intros flat_smem H_sbindings H_map_option. simpl in H_map_option. injection H_map_option as H_map_option. rewrite <- H_map_option. simpl. reflexivity.
   - intros flat_smem H_sbindings H_map_option.
@@ -435,10 +430,10 @@ Proof.
                     rewrite <- H_map_option_1;
                     simpl;
 
-                    pose proof (eval_sexpr_snd sb offset stk mem strg ctx ops flat_sb flat_offset H_sbindings E_sstack_val_to_sexpr_offset) as H_eval_sexpr_snd_offset;
+                    pose proof (eval_sexpr_snd sb maxidx offset stk mem strg ctx ops flat_sb flat_offset H_sbindings E_sstack_val_to_sexpr_offset) as H_eval_sexpr_snd_offset;
                     rewrite H_eval_sexpr_snd_offset;
 
-                    pose proof (eval_sexpr_snd sb value stk mem strg ctx ops flat_sb flat_value H_sbindings E_sstack_val_to_sexpr_value) as H_eval_sexpr_snd_value;
+                    pose proof (eval_sexpr_snd sb maxidx value stk mem strg ctx ops flat_sb flat_value H_sbindings E_sstack_val_to_sexpr_value) as H_eval_sexpr_snd_value;
                     rewrite H_eval_sexpr_snd_value;
 
                     pose proof (IHsmem' flat_smem' H_sbindings  H_map_option_2) as IHsmem'_1;
@@ -449,13 +444,13 @@ Qed.
 Lemma eval_flat_smemory_snd:
   forall sst fsst stk mem strg ctx ops,
     sstate_to_flat_sstate sst = Some fsst ->
-    eval_flat_smemory stk mem strg ctx fsst ops = eval_smemory stk mem strg ctx sst ops.
+    eval_flat_smemory (get_memory_fsst fsst) stk mem strg ctx ops = eval_smemory (get_memory_sst sst) (get_maxidx_smap (get_smap_sst sst)) (get_bindings_smap (get_smap_sst sst)) stk mem strg ctx ops.
 Proof.
   intros sst fsst stk mem strg ctx ops H_sst_to_fsst.
   unfold eval_flat_smemory.
   unfold eval_smemory.
   unfold sstate_to_flat_sstate in H_sst_to_fsst.
-  destruct (get_smap_sst sst) as [maxid sb] eqn:E_get_smap.
+  destruct (get_smap_sst sst) as [maxidx sb] eqn:E_get_smap.
   unfold sstate_to_flat_sstate in H_sst_to_fsst.
   destruct (bindings_to_flat_bindings sb) as [flat_sb|] eqn:E_bindings; try discriminate.
   destruct (sstack_to_flat_sstack sst flat_sb) as [flat_sstk|] eqn:E_flat_sstk; try discriminate.
@@ -465,20 +460,20 @@ Proof.
   rewrite <- H_sst_to_fsst.
   simpl.
   unfold smemory_to_flat_smemory in E_flat_smem.
-  pose proof (eval_flat_smemory_map sb flat_sb stk mem strg ctx ops (get_memory_sst sst) flat_smem E_bindings E_flat_smem) as H_eval_flat_smemory_map.
+  pose proof (eval_flat_smemory_map sb maxidx flat_sb stk mem strg ctx ops (get_memory_sst sst) flat_smem E_bindings E_flat_smem) as H_eval_flat_smemory_map.
   rewrite H_eval_flat_smemory_map.
   reflexivity.
 Qed.
 
 Lemma eval_flat_sstorage_map:
-  forall sb flat_sb stk mem strg ctx ops sstrg flat_sstrg,
+  forall sb maxidx flat_sb stk mem strg ctx ops sstrg flat_sstrg,
     bindings_to_flat_bindings sb = Some flat_sb ->
     map_option (eval_common.EvalCommon.instantiate_storage_update (fun sv : sstack_val => sstack_val_to_sexpr sv flat_sb)) sstrg = Some flat_sstrg ->
 
   map_option (eval_common.EvalCommon.instantiate_storage_update (fun sv : sexpr => eval_sexpr sv stk mem strg ctx ops)) flat_sstrg =
-    map_option (eval_common.EvalCommon.instantiate_storage_update (fun sv : sstack_val => eval_sstack_val sv stk mem strg ctx sb ops)) sstrg.
+    map_option (eval_common.EvalCommon.instantiate_storage_update (fun sv : sstack_val => eval_sstack_val sv stk mem strg ctx maxidx sb ops)) sstrg.
 Proof. (* it is the same as eval_flat_smemory_map *)
-  intros sb flat_sb stk mem strg ctx ops.
+  intros sb maxidx flat_sb stk mem strg ctx ops.
   induction sstrg as [|u sstrg' IHsstrg'].
   - intros flat_sstrg H_sbindings H_map_option. simpl in H_map_option. injection H_map_option as H_map_option. rewrite <- H_map_option. simpl. reflexivity.
   - intros flat_sstrg H_sbindings H_map_option.
@@ -498,10 +493,10 @@ Proof. (* it is the same as eval_flat_smemory_map *)
     rewrite <- H_map_option_1.
     simpl.
     
-    pose proof (eval_sexpr_snd sb key stk mem strg ctx ops flat_sb flat_key H_sbindings E_sstack_val_to_sexpr_key) as H_eval_sexpr_snd_key.
+    pose proof (eval_sexpr_snd sb maxidx key stk mem strg ctx ops flat_sb flat_key H_sbindings E_sstack_val_to_sexpr_key) as H_eval_sexpr_snd_key.
     rewrite H_eval_sexpr_snd_key.
     
-    pose proof (eval_sexpr_snd sb value stk mem strg ctx ops flat_sb flat_value H_sbindings E_sstack_val_to_sexpr_value) as H_eval_sexpr_snd_value.
+    pose proof (eval_sexpr_snd sb maxidx value stk mem strg ctx ops flat_sb flat_value H_sbindings E_sstack_val_to_sexpr_value) as H_eval_sexpr_snd_value.
     rewrite H_eval_sexpr_snd_value.
     
     pose proof (IHsstrg' flat_sstrg' H_sbindings  H_map_option_2) as IHsstrg'_1.
@@ -512,13 +507,13 @@ Qed.
 Lemma eval_flat_sstorage_snd:
   forall sst fsst stk mem strg ctx ops,
     sstate_to_flat_sstate sst = Some fsst ->
-    eval_flat_sstorage stk mem strg ctx fsst ops = eval_sstorage stk mem strg ctx sst ops.
+    eval_flat_sstorage (get_storage_fsst fsst) stk mem strg ctx ops = eval_sstorage (get_storage_sst sst) (get_maxidx_smap (get_smap_sst sst)) (get_bindings_smap (get_smap_sst sst)) stk mem strg ctx ops.
 Proof.
   intros sst fsst stk mem strg ctx ops H_sst_to_fsst.
   unfold eval_flat_sstorage.
   unfold eval_sstorage.
   unfold sstate_to_flat_sstate in H_sst_to_fsst.
-  destruct (get_smap_sst sst) as [maxid sb] eqn:E_get_smap.
+  destruct (get_smap_sst sst) as [maxidx sb] eqn:E_get_smap.
   unfold sstate_to_flat_sstate in H_sst_to_fsst.
   destruct (bindings_to_flat_bindings sb) as [flat_sb|] eqn:E_bindings; try discriminate.
   destruct (sstack_to_flat_sstack sst flat_sb) as [flat_sstk|] eqn:E_flat_sstk; try discriminate.
@@ -528,7 +523,7 @@ Proof.
   rewrite <- H_sst_to_fsst.
   simpl.
   unfold sstorage_to_flat_sstorage in E_flat_smem.
-  pose proof (eval_flat_sstorage_map sb flat_sb stk mem strg ctx ops (get_storage_sst sst) flat_sstrg E_bindings E_flat_sstrg) as H_eval_flat_sstorage_map.
+  pose proof (eval_flat_sstorage_map sb maxidx flat_sb stk mem strg ctx ops (get_storage_sst sst) flat_sstrg E_bindings E_flat_sstrg) as H_eval_flat_sstorage_map.
   rewrite H_eval_flat_sstorage_map.
   reflexivity.
 Qed.
@@ -539,9 +534,13 @@ Lemma eval_flat_sstate_snd:
     eval_flat_sstate st fsst ops = eval_sstate st sst ops.
 Proof.
   intros sst fsst st ops H_sst_to_fsst.
+
+  pose proof (sst_to_fsst_instk_height sst fsst H_sst_to_fsst) as H_instk_height.
   unfold eval_flat_sstate.
   unfold eval_sstate.
 
+  rewrite H_instk_height.
+  
   pose proof (eval_flat_sstack_snd sst fsst (get_stack_st st) (get_memory_st st) (get_storage_st st) (get_context_st st) ops H_sst_to_fsst) as H_eval_flat_sstack_snd.
   rewrite H_eval_flat_sstack_snd.
 
