ver2/memory_ops_solvers.v
@@ -31,7 +31,7 @@ Import SymbolicStateEval.
 Require Import FORVES.valid_symbolic_state.
 Import ValidSymbolicState.
 
-Module LoadSolvers.
+Module MemoryOpsSolvers.
 
 (* sv smem instk_height m ops -> load_res *)
 Definition mload_solver_type := sstack_val -> smemory -> nat -> smap -> stack_op_instr_map -> smap_value.
@@ -60,36 +60,6 @@ Definition mload_solver_snd (mload_solver: mload_solver_type) :=
   mload_solver_valid_res mload_solver /\ mload_solver_correct_res mload_solver.
 
 
-(* sv smem instk_height m ops -> load_res *)
-Definition sload_solver_type := sstack_val -> sstorage -> nat -> smap -> stack_op_instr_map -> smap_value.
-
-Definition sload_solver_valid_res (sload_solver: sload_solver_type) :=
-  forall m sstrg skey instk_height smv ops,
-    valid_sstorage instk_height (get_maxidx_smap m) sstrg -> (* The storage is valid *)
-    valid_sstack_value instk_height (get_maxidx_smap m) skey -> (* The key is valid *)    
-    sload_solver skey sstrg instk_height m ops = smv ->
-    valid_smap_value instk_height (get_maxidx_smap m) ops smv.
-
-Definition sload_solver_correct_res (sload_solver: sload_solver_type) :=
-  forall m sstrg skey instk_height smv ops idx1 m1,
-    valid_sstorage instk_height (get_maxidx_smap m) sstrg -> (* The storage is valid *)
-    valid_sstack_value instk_height (get_maxidx_smap m) skey -> (* The key is valid *)    
-    sload_solver skey sstrg instk_height m ops = smv -> (* The value was resolved *)
-    add_to_smap m smv = (idx1, m1) ->
-    exists idx2 m2,
-      add_to_smap m (SymSLOAD skey sstrg) = (idx2, m2) /\
-      forall stk mem strg ctx,
-      exists v,
-        eval_sstack_val(FreshVar idx1) stk mem strg ctx (get_maxidx_smap m1) (get_bindings_smap m1) ops = Some v /\
-          eval_sstack_val(FreshVar idx2) stk mem strg ctx (get_maxidx_smap m2) (get_bindings_smap m2) ops = Some v.
-
-Definition sload_solver_snd (sload_solver: sload_solver_type) :=
-  sload_solver_valid_res sload_solver /\ sload_solver_correct_res sload_solver.
-
-
-(* Abstractions for memory/storage operations during symbolic execution *)
-
-
 (* u smem instk_height m ops -> smem' *)
 Definition smemory_updater_type := memory_update sstack_val -> smemory -> nat -> smap -> stack_op_instr_map -> smemory.
 
@@ -115,29 +85,4 @@ Definition smemory_updater_correct_res (smemory_updater: smemory_updater_type) :
 Definition smemory_updater_snd (smemory_updater: smemory_updater_type) :=
   smemory_updater_valid_res smemory_updater /\ smemory_updater_correct_res smemory_updater.
 
-
-(* u smem instk_height m ops -> strg' *)
-Definition sstorage_updater_type := storage_update sstack_val -> sstorage -> nat -> smap -> stack_op_instr_map -> sstorage.
-
-Definition sstorage_updater_valid_res (sstorage_updater: sstorage_updater_type) :=
-  forall m sstrg sstrg' u instk_height ops,
-    valid_sstorage instk_height (get_maxidx_smap m) sstrg -> (* The storage is valid *)
-    valid_sstorage_update instk_height (get_maxidx_smap m) u -> (* The update is valid *)    
-    sstorage_updater u sstrg instk_height m ops = sstrg' ->
-    valid_sstorage instk_height (get_maxidx_smap m) sstrg'. (* The new storage is valid *)
-
-Definition sstorage_updater_correct_res (sstorage_updater: sstorage_updater_type) :=
-  forall m sstrg sstrg' u instk_height ops,
-    valid_sstorage instk_height (get_maxidx_smap m) sstrg -> (* The storage is valid *)
-    valid_sstorage_update instk_height (get_maxidx_smap m) u -> (* The update is valid *)    
-    sstorage_updater u sstrg instk_height m ops = sstrg' ->
-    forall stk mem strg ctx,
-      exists strg1 strg2,
-        eval_sstorage (u::sstrg) (get_maxidx_smap m) (get_bindings_smap m) stk mem strg ctx ops = Some strg1 /\
-          eval_sstorage sstrg' (get_maxidx_smap m) (get_bindings_smap m) stk mem strg ctx ops = Some strg2 /\
-          eq_storage strg1 strg2.
-
-Definition sstorage_updater_snd (sstorage_updater: sstorage_updater_type) :=
-  sstorage_updater_valid_res sstorage_updater /\ sstorage_updater_correct_res sstorage_updater.
-
-End LoadSolvers.
+End MemoryOpsSolvers.
