ver2/storage_ops_solvers.v
@@ -1,0 +1,89 @@
+Require Import Arith.  
+Require Import Nat.
+Require Import Bool.
+Require Import bbv.Word.
+Require Import Coq.NArith.NArith.
+Require Import List.
+Import ListNotations.
+Require Import Coq.Logic.FunctionalExtensionality.
+
+Require Import FORVES.constants.
+Import Constants.
+
+Require Import FORVES.program.
+Import Program.
+
+Require Import FORVES.execution_state.
+Import ExecutionState.
+
+Require Import FORVES.stack_operation_instructions.
+Import StackOpInstrs.
+
+Require Import FORVES.misc.
+Import Misc.
+
+Require Import FORVES.symbolic_state.
+Import SymbolicState.
+
+Require Import FORVES.symbolic_state_eval.
+Import SymbolicStateEval.
+
+Require Import FORVES.valid_symbolic_state.
+Import ValidSymbolicState.
+
+Module StorageOpsSolvers.
+
+
+
+(* sv smem instk_height m ops -> load_res *)
+Definition sload_solver_type := sstack_val -> sstorage -> nat -> smap -> stack_op_instr_map -> smap_value.
+
+Definition sload_solver_valid_res (sload_solver: sload_solver_type) :=
+  forall m sstrg skey instk_height smv ops,
+    valid_sstorage instk_height (get_maxidx_smap m) sstrg -> (* The storage is valid *)
+    valid_sstack_value instk_height (get_maxidx_smap m) skey -> (* The key is valid *)    
+    sload_solver skey sstrg instk_height m ops = smv ->
+    valid_smap_value instk_height (get_maxidx_smap m) ops smv.
+
+Definition sload_solver_correct_res (sload_solver: sload_solver_type) :=
+  forall m sstrg skey instk_height smv ops idx1 m1,
+    valid_sstorage instk_height (get_maxidx_smap m) sstrg -> (* The storage is valid *)
+    valid_sstack_value instk_height (get_maxidx_smap m) skey -> (* The key is valid *)    
+    sload_solver skey sstrg instk_height m ops = smv -> (* The value was resolved *)
+    add_to_smap m smv = (idx1, m1) ->
+    exists idx2 m2,
+      add_to_smap m (SymSLOAD skey sstrg) = (idx2, m2) /\
+      forall stk mem strg ctx,
+      exists v,
+        eval_sstack_val(FreshVar idx1) stk mem strg ctx (get_maxidx_smap m1) (get_bindings_smap m1) ops = Some v /\
+          eval_sstack_val(FreshVar idx2) stk mem strg ctx (get_maxidx_smap m2) (get_bindings_smap m2) ops = Some v.
+
+Definition sload_solver_snd (sload_solver: sload_solver_type) :=
+  sload_solver_valid_res sload_solver /\ sload_solver_correct_res sload_solver.
+
+
+(* u sstrg instk_height m ops -> strg' *)
+Definition sstorage_updater_type := storage_update sstack_val -> sstorage -> nat -> smap -> stack_op_instr_map -> sstorage.
+
+Definition sstorage_updater_valid_res (sstorage_updater: sstorage_updater_type) :=
+  forall m sstrg sstrg' u instk_height ops,
+    valid_sstorage instk_height (get_maxidx_smap m) sstrg -> (* The storage is valid *)
+    valid_sstorage_update instk_height (get_maxidx_smap m) u -> (* The update is valid *)    
+    sstorage_updater u sstrg instk_height m ops = sstrg' ->
+    valid_sstorage instk_height (get_maxidx_smap m) sstrg'. (* The new storage is valid *)
+
+Definition sstorage_updater_correct_res (sstorage_updater: sstorage_updater_type) :=
+  forall m sstrg sstrg' u instk_height ops,
+    valid_sstorage instk_height (get_maxidx_smap m) sstrg -> (* The storage is valid *)
+    valid_sstorage_update instk_height (get_maxidx_smap m) u -> (* The update is valid *)    
+    sstorage_updater u sstrg instk_height m ops = sstrg' ->
+    forall stk mem strg ctx,
+      exists strg1 strg2,
+        eval_sstorage (u::sstrg) (get_maxidx_smap m) (get_bindings_smap m) stk mem strg ctx ops = Some strg1 /\
+          eval_sstorage sstrg' (get_maxidx_smap m) (get_bindings_smap m) stk mem strg ctx ops = Some strg2 /\
+          eq_storage strg1 strg2.
+
+Definition sstorage_updater_snd (sstorage_updater: sstorage_updater_type) :=
+  sstorage_updater_valid_res sstorage_updater /\ sstorage_updater_correct_res sstorage_updater.
+
+End StorageOpsSolvers.
