ver2/symbolic_execution_soundness.v
@@ -37,8 +37,11 @@ Import ValidSymbolicState.
 Require Import FORVES.concrete_interpreter.
 Import ConcreteInterpreter.
 
-Require Import FORVES.load_solvers.
-Import LoadSolvers.
+Require Import FORVES.memory_ops_solvers.
+Import MemoryOpsSolvers.
+
+Require Import FORVES.storage_ops_solvers.
+Import StorageOpsSolvers.
 
 Module SymbolicExecutionSoundness.
 
