ver2/symbolic_state_cmp.v
@@ -1,0 +1,108 @@
+
+Require Import Arith.
+Require Import Nat.
+Require Import Bool.
+Require Import bbv.Word.
+Require Import Coq.NArith.NArith.
+Require Import List.
+Import ListNotations.
+
+Require Import FORVES.constants.
+Import Constants.
+
+Require Import FORVES.program.
+Import Program.
+
+Require Import FORVES.execution_state.
+Import ExecutionState.
+
+Require Import FORVES.stack_operation_instructions.
+Import StackOpInstrs.
+
+Require Import FORVES.misc.
+Import Misc.
+
+Require Import FORVES.symbolic_state.
+Import SymbolicState.
+
+Require Import FORVES.symbolic_state_eval.
+Import SymbolicStateEval.
+
+
+Require Import FORVES.concrete_interpreter.
+Import ConcreteInterpreter.
+
+Require Import FORVES.eval_common.
+Import EvalCommon.
+
+Module FlatSymbolicStateCmp.
+
+
+Fixpoint smap_val_cmp (smem_cmp: smemory_cmp_type) (sstrg_cmp: sstorage_cmp_type) (sha3_cmp: sha3_cmp_type) (d :nat) (smv1 smv2: smap_value) (instk_height: nat) (sb1 sb2 : sbindings) (ops: stack_op_instr_map) : bool :=
+  match d with
+  | 0 => false
+  | S d' =>
+      match smv1, smv2 with
+      | SymBasicVal (Val v1), SymBasicVal (Val v2) => weqb v1 v2
+      | SymBasicVal (InStackVar n1), SymBasicVal (InStackVar n2) => (andb (n1 =? n2) (andb (n1 <? instk_height) (n2 <? instk_height)))
+      | SymBasicVal (FreshVar n), _ => 
+           match sb1 with
+           | [] => false
+           | (key,smv)::sb1' =>
+               if key =? n then
+                 smap_val_cmp smem_cmp sstrg_cmp sha3_cmp d' smv smv2 instk_height sb1' sb2 ops
+               else
+                 smap_val_cmp smem_cmp sstrg_cmp sha3_cmp d' smv1 smv2 instk_height sb1' sb2 ops
+           end
+      | _, SymBasicVal (FreshVar n) => 
+           match sb2 with
+           | [] => false
+           | (key,smv)::sb2' =>
+               if key =? n then
+                 smap_val_cmp smem_cmp sstrg_cmp sha3_cmp d' smv1 smv instk_height sb1 sb2' ops
+               else
+                 smap_val_cmp smem_cmp sstrg_cmp sha3_cmp d' smv1 smv2 instk_height sb1 sb2' ops
+           end
+      | SymPUSHTAG v1, SymPUSHTAG v2 => (v1 =? v2)%N
+      | SymOp label1 args1, SymOp label2 args2 =>
+          if ( label1 =?i label2 ) then
+            match ops label1 with
+            | OpImp nargs f H_comm H_ctx_ind =>
+                if (andb (length args1 =? nargs) (length args2 =? nargs) ) then
+                  match (fold_right_two_lists (fun e1 e2 => smap_val_cmp smem_cmp sstrg_cmp sha3_cmp d' (SymBasicVal e1) (SymBasicVal e2) instk_height sb1 sb2 ops) args1 args2) with
+                  | true => true
+                  | false => match H_comm with
+                             | None => false
+                             | Some Comm_Proof =>
+                                 match args1, args2 with
+                                 | [a1;a2], [b1;b2] => andb (smap_val_cmp smem_cmp sstrg_cmp sha3_cmp d' (SymBasicVal a1) (SymBasicVal b2) instk_height sb1 sb2 ops)
+                                                            (smap_val_cmp smem_cmp sstrg_cmp sha3_cmp d' (SymBasicVal a2) (SymBasicVal b1) instk_height sb1 sb2 ops) 
+                                 | _, _ => false
+                                 end
+                             end
+                  end
+            else
+              false
+            end
+          else
+            false
+      | SymMLOAD offset1 smem1, SymMLOAD offset2 smem2 =>
+          if (smap_val_cmp smem_cmp sstrg_cmp sha3_cmp d' (SymBasicVal offset1) (SymBasicVal offset1) instk_height sb1 sb2 ops) then
+            smem_cmp (fun a b => false) smem1 smem2
+          else
+            false               
+      | SymSLOAD key1 sstrg1, SymSLOAD key2 sstrg2 => 
+          if (smap_val_cmp smem_cmp sstrg_cmp sha3_cmp d' (SymBasicVal key1) (SymBasicVal key2) instk_height sb1 sb2 ops) then
+            sstrg_cmp (fun a b => false) sstrg1 sstrg2
+          else
+            false
+      | SymSHA3 offset1 size1 smem1, SymSHA3 offset2 size2 smem2 =>
+          sha3_cmp (fun a b => false) offset1 size1 smem1 offset2 size2 smem2
+      | _, _ => false
+      end
+  end.
+
+
+End FlatSymbolicStateCmp.
+
+  
